isabelle/Substitution.thy
@@ -1,0 +1,7 @@
+theory Substitution
+  imports Main AbstractBindingTrees
+begin
+
+
+
+end
